examples/httpProtocolMock/main.c
@@ -1,0 +1,110 @@
+#include <stdio.h>
+#include <stdlib.h>
+#include <sys/fcntl.h>
+#include <sys/socket.h>
+#include <sys/types.h>
+#include <netinet/in.h>
+#include <netdb.h>
+#include <string.h>
+#include <unistd.h>
+#include <errno.h>
+
+#include "HttpServer.h"
+
+static int sockfd;
+static int new_sockfd;
+
+void http(int sockfd) {
+  char request[2048] = {0};
+  char response[2048] = {0};
+
+  if ((read(sockfd, request, sizeof(request))) <= 0) {
+    perror("reading a request.");
+    return;
+  }
+
+  httpServerLib((char *) request, response);
+
+  if (write(sockfd, response, strlen(response)) != strlen(response)) {
+    perror("writing a response .");
+    return;
+  }
+
+  if (close(sockfd) == -1) {
+    perror("close socket in http()");
+  }
+
+  return;
+}
+
+void signalHandler(int signal){
+    fprintf(stderr,"\nEXIT SIGNAL:%d\n",signal);
+
+    if (close(sockfd) == -1) {
+        perror("close sockfd in signalHandler().");
+    }
+
+    puts("HTTP Server Stop.");
+    exit(EXIT_SUCCESS);
+}
+
+int main(int argc, char *argv[]) {
+
+  signal( SIGINT, signalHandler);
+
+  puts("Listening on http://localhost");
+
+  int writer_len;
+
+  struct sockaddr_in reader_addr;
+  struct sockaddr_in writer_addr;
+
+  memset(&reader_addr, 0, sizeof(reader_addr));
+  memset(&writer_addr, 0, sizeof(writer_addr));
+
+  reader_addr.sin_family      = AF_INET;
+  reader_addr.sin_addr.s_addr = htonl(INADDR_ANY);
+  reader_addr.sin_port        = htons(80);
+
+  if ((sockfd = socket(AF_INET, SOCK_STREAM, 0)) < 0) {
+      perror("socket()");
+      return 1;
+  }
+
+  int optval = 1;
+  if (setsockopt(sockfd, SOL_SOCKET, SO_REUSEADDR, (const char *)&optval, sizeof(optval)) == -1) {
+      perror("setsockopt()");
+      return 1;
+  }
+
+  if (bind(sockfd, (struct sockaddr *)&reader_addr, sizeof(reader_addr)) < 0) {
+      perror("bind()");
+      if (close(sockfd) == -1) {
+        perror("close socket.");
+      }
+      return 1;
+  }
+
+  if (listen(sockfd, 5) < 0) {
+      perror("listen()");
+      if (close(sockfd) == -1) {
+        perror("close socket.");
+      }
+      return 1;
+  }
+
+  while(1) {
+      if ((new_sockfd = accept(sockfd, (struct sockaddr *)&writer_addr, (socklen_t *)&writer_len)) < 0) {
+          perror("accepting a socket.");
+
+          if (close(sockfd) == -1) {
+              perror("close sockfd.");
+          }
+          break;
+      }
+
+      http(new_sockfd);
+  }
+
+  return 1;
+}
